lakefile.lean
@@ -22,5 +22,8 @@ package OperatorKO7 where
 lean_lib OperatorKO7 where
   roots := #[`OperatorKO7]
 
+lean_exe verifyTpdbExport where
+  root := `VerifyTpdbExport
+
 require mathlib from git "https://github.com/leanprover-community/mathlib4.git" @ "632465e4b02cb70a5dfa4cfe15468e8a62c2bd85"
 
